% !TEX root = ../main.tex

\chapter{Beyond Interpolation: Proofs}~\label{app:beyond-interpolation}

\regularizedWGC*
\begin{proof}
   By definition of the \( L_2 \)-regularized oracle \( \oracle{}_2 \),
   \begin{align*}
       \Ek\sbr{\norm{\nabla F(\w, \zk)}^2} &= \Ek\sbr{\norm{\grad(\w, \zk) + \lambda \w}^2}.
       \intertext{Young's inequality for products and the weak growth condition imply}
       \Ek\sbr{\norm{\nabla F(\w, \zk)}^2}&\leq \Ek\sbr{2 \norm{\grad(\w, \zk)}^2 + 2 \lambda^2 \norm{\w}^2}\\
                                                     &\leq 4 \rho L \rbr{f(\w) - f(\wbar)} + 2 \lambda^2 \norm{\w}^2.
       \intertext{We now proceed in cases depending on the degree of regularization. If \( \lambda \leq \rho L \),}
       \implies  \Ek\sbr{\norm{\nabla F(\w, \zk)}^2} &\leq 4 \rho L \rbr{f(\w) - f(\wbar) + \frac{\lambda^2}{2 \rho L} \norm{\w}^2}\\
                                                              &\leq 4 \rho L \rbr{f(\w) - f(\wbar) + \frac{\lambda}{2} \norm{\w}^2}\\ 
                                                              &= 4 \rho L \rbr{F(w) - f(\wbar)}.
                                                              \intertext{On the other hand, if \( \lambda > \rho L \), }
       \implies \Ek\sbr{\norm{\nabla F(\w, \zk)}^2} &\leq 4 \lambda \rbr{f(\w) - f(\wbar) + \frac{\lambda}{2} \norm{\w}^2}\\
                                                              &= 4 \lambda \rbr{F(\w) - f(\wbar)}. 
                                                              \intertext{Combining the two cases yields}
        \Ek\sbr{\norm{\nabla F(\w, \zk)}^2} &\leq 4 \max\cbr{\rho L, \lambda}\rbr{F(\w) - f(\wbar)}.
       \intertext{Let \( \delta = \mu \) if \( f \) is \( \mu \)-strongly-convex and set \( \delta = -L \) otherwise. 
                  Strong-convex (or smoothness if \( \delta = -L \)) implies \( f(\wbar) \geq f(\wopt) + \abr{\grad(\wopt), \wbar - \wopt} + \frac{\delta}{2}\norm{\wbar - \wopt}^2 \). Subsituting this into the bound gives}
       \Ek\sbr{\norm{\nabla F(\w, \zk)}^2} &\leq 4 \max\cbr{\rho L, \lambda}\rbr{F(\w) - f(\wopt) - \abr{\grad(\wopt), \wbar - \wopt} - \frac{\delta}{2}\norm{\wbar - \wopt}^2}\\
       \intertext{Recall that \( \wopt \) minimizes the regularized function \( F \). Then, by first-order optimality conditions, \( \grad(\wopt) = - \lambda \wopt \) and we obtain} 
       \Ek\sbr{\norm{\nabla F(\w, \zk)}^2} &\leq 4 \max\cbr{\rho L, \lambda} \rbr{F(\w) - f(\wopt) + \abr{\lambda \wopt, \wbar - \wopt} - \frac{\delta}{2}\norm{\wbar - \wopt}^2 }\\
                                                     &= 4 \max\cbr{\rho L, \lambda} \rbr{F(\w) - f(\wopt) - \lambda \norm{\wopt}^2  + \lambda \abr{\wopt, \wbar} - \frac{\delta}{2}\norm{\wbar - \wopt}^2}\\
                                                     &=  4 \max\cbr{\rho L, \lambda} \rbr{F(\w) - F(\wopt) - \frac{\lambda}{2} \norm{\wopt}^2 + \lambda \abr{\wopt, \wbar} - \frac{\delta}{2}\norm{\wbar - \wopt}^2}\\
                                                     &= 4 \max\cbr{\rho L, \lambda} \rbr{F(\w) - F(\wopt) - \frac{\lambda + \delta}{2} \norm{\wopt - \wbar}^2 + \frac{\lambda}{2} \norm{\wbar}^2}.
   \end{align*} 
   Substituting in the appropriate value for \( \delta \) completes the proof.
\end{proof}

\section{Convergence for \( L_2 \)-Regularized Convex Functions}~\label{app:regularized-convex}

\sgdReguarlizedWGC*
\begin{proof}
    \begin{align*}
        \norm{\wkk - \wopt}^2 &= \norm{\wk - \eta \nabla F(\wk, \zk) - \wopt}^2\\
                              &= \eta^2 \norm{\nabla F(\wk, \zk)}^2 - 2 \eta \abr{\nabla F(\wk, \zk), \wk - \wopt} + \norm{\wk - \wopt}^2.
                              \intertext{Taking expectations with respect to \( \Ek \),}
        \implies \Ek\sbr{\norm{\wkk - \wopt}^2} &= \eta^2 \Ek \sbr{\norm{\nabla F(\wk, \zk)}^2} - 2 \eta \Ek\sbr{\abr{\nabla F(\wk, \zk), \wk - \wopt}} + \norm{\wk - \wopt}^2\\
                                                &= \eta^2 \Ek\sbr{\norm{\nabla F(\wk, \zk)}^2} - 2 \eta \abr{\nabla F(\wk), \wk - \wopt} + \norm{\wk - \wopt}^2.
                                                \intertext{Let \( C = 4 \eta^2 \max\cbr{\rho L, \lambda} \rbr{ \frac{\lambda}{2} \norm{\wbar}^2 - \frac{\lambda + \mu}{2} \norm{\wopt - \wbar}^2} \). Then \autoref{lemma:regularized-wgc} implies}
        \Ek\sbr{\norm{\wkk - \wopt}^2} &\leq 4 \eta^2 \max\cbr{\rho L, \lambda} \rbr{F(\wk) - F(\wopt)} - 2 \eta \abr{\nabla F(\wk), \wk - \wopt} + \norm{\wk - \wopt}^2 + C\\
        \intertext{Using \( (\mu + \lambda) \)-strong-convexity of \( f \),}
        \implies  \Ek\sbr{\norm{\wkk - \wopt}^2} &\leq \frac{2 \eta^2 \max\cbr{\rho L, \lambda}}{\mu + \lambda} \norm{\nabla F(\wk)}^2 - 2 \eta \abr{\nabla F(\wk), \wk - \wopt} + \norm{\wk - \wopt}^2 \\ & \hspace{4em} + C.
        \intertext{Coercivity of the gradient (\autoref{lemma:coercivity}) now implies} 
        \Ek\sbr{\norm{\wkk - \wopt}^2} &\leq \frac{2 \eta^2 \max\cbr{\rho L, \lambda}}{\mu + \lambda} \norm{\nabla F(\wk)}^2 - 2 \eta \bigg( \frac{(\mu + \lambda)(L + \lambda)}{(\mu + \lambda) + (L + \lambda)} \norm{\wk - \wopt}^2 \\ & \hspace{5em} + \frac{1}{(\mu + \lambda) + (L + \lambda)} \norm{\nabla F(\wk)}^2 \bigg) + C\\
                                       &= 2 \eta \rbr{\frac{\eta \max\cbr{\rho L, \lambda}}{\mu + \lambda} - \frac{1}{(\mu + \lambda) + (L + \lambda)}} \norm{\nabla F(\wk)}^2 \\ & \hspace{5em} + \rbr{1 - \frac{2 \eta (\mu + \lambda)(L + \lambda)}{(\mu + \lambda) + (L + \lambda)}} \norm{\wk - \wopt}^2 + C.  
                                       \intertext{If \( \eta \leq \frac{\mu + \lambda}{\max\cbr{\rho L, \lambda}\rbr{(\mu + \lambda) + (L + \lambda)}} \) then we obtain}
        \Ek\sbr{\norm{\wkk - \wopt}^2} &\leq \rbr{1 - \frac{2 \eta (\mu + \lambda)(L + \lambda)}{(\mu + \lambda) + (L + \lambda)}} \norm{\wk - \wopt}^2 + C.
        \intertext{Let \( \delta =  \frac{2 \eta (\mu + \lambda)(L + \lambda)}{(\mu + \lambda) + (L + \lambda)} \). Taking expectations and recursing on this inequality,}
        \implies \E\sbr{\norm{\wkk - \wopt}^2} &\leq \rbr{1 - \delta}^k \norm{\w_0 - \wopt}^2 + C \sum_{l=0}^{k-1}  \rbr{1 - \delta}^l\\
                                               & = \rbr{1 - \delta}^k \norm{\w_0 - \wopt}^2 + C \rbr{\frac{1 - {(1 - \delta)}^k}{\delta}}\\
                                               &\leq  \rbr{1 - \delta}^k \norm{\w_0 - \wopt}^2 + \frac{C}{\delta}.
                                               \intertext{Letting \( \gamma = \frac{C}{\delta} =  \frac{\eta \max\cbr{\rho L, \lambda} \sbr{(\mu + \lambda) + (L + \lambda)}}{(\mu + \lambda)(L + \lambda)}\) and subsituting in the value of \( \delta \) gives the final result:}
        \implies \E\sbr{\norm{\wkk - \wopt}^2} &\leq \rbr{1 - \frac{2 \eta (\mu + \lambda)(L + \lambda)}{(\mu + \lambda) + (L + \lambda)}}^k \norm{\w_0 - \wopt}^2 + \frac{\gamma}{2}\rbr{\lambda \norm{\wbar}^2 - \rbr{\lambda + \mu}\norm{\wopt - \wbar}^2}.
    \end{align*}
\end{proof}
